Finish with matrices definitions and theorems.

src/TraverseOpImpl.v
@@ -35,7 +35,7 @@ Section translate.
 
   Lemma vertex_ltb_vertices_sub v
     (HIn : In v V) : v < vertices_sup.
-  Proof.
+  Proof using.
     unfold vertices_sup.
     apply ltb_succ.
     change (v <= \sup_(v0 \in V) v0) with
@@ -45,7 +45,7 @@ Section translate.
 
   Lemma edge_ltb_edges_sub e
     (HIn : In e E) : e < edges_sup.
-  Proof.
+  Proof using.
     unfold edges_sup.
     apply ltb_succ.
     change (e <= \sup_(e0\in E) e0) with
@@ -71,14 +71,14 @@ Section translate.
                | None => true
                end.
 
-  Theorem adj_matrix_of_edge_spec e l i j :
+  Lemma adj_matrix_of_edge_spec e l i j :
     adj_matrix_of_edge l e i j <->
       Path.matches_direction G i j e Pattern.OUT /\
       match l with
       | Some l => elabel G e = l
       | None => True
       end.
-  Proof.
+  Proof using.
     unfold adj_matrix_of_edge.
     unfold is_true; desf.
     all: repeat rewrite Bool.andb_true_iff.
@@ -90,32 +90,32 @@ Section translate.
   Definition adj_matrix (l : option label) : adj_mat_ty :=
     (\sum_(e \in E) (adj_matrix_of_edge l e)).
 
-  Theorem adj_matrix_spec_OUT l i j :
+  Lemma adj_matrix_spec_OUT l i j :
     adj_matrix l i j <-> exists e, In e E /\
       Path.matches_direction G i j e Pattern.OUT /\
       match l with
       | Some l => elabel G e = l
       | None => True
       end.
-  Proof.
+  Proof using.
     unfold adj_matrix.
     setoid_rewrite <- adj_matrix_of_edge_spec.
     rewrite <- is_true_sup.
     now rewrite <- mx_sup.
   Qed.
 
-  Theorem adj_matrix_spec_IN l i j :
+  Lemma adj_matrix_spec_IN l i j :
     adj_matrix l j i <-> exists e, In e E /\
       Path.matches_direction G i j e Pattern.IN /\
       match l with
       | Some l => elabel G e = l
       | None => True
       end.
-  Proof.
+  Proof using.
     simpl. apply adj_matrix_spec_OUT.
   Qed.
 
-  Theorem adj_matrix_spec_BOTH l i j :
+  Lemma adj_matrix_spec_BOTH l i j :
     adj_matrix l i j || adj_matrix l j i <->
       exists e, In e E /\
         Path.matches_direction G i j e Pattern.BOTH /\
@@ -123,7 +123,7 @@ Section translate.
         | Some l => elabel G e = l
         | None => True
         end.
-  Proof.
+  Proof using.
     unfold is_true.
     rewrite Bool.orb_true_iff.
     change (?b = true) with (is_true b).
@@ -132,56 +132,12 @@ Section translate.
     split; ins; desf; eauto.
   Qed.
 
-  Definition inc_mat_ty := bmx vertices_sup edges_sup.
-
-  Definition inc_matrix : inc_mat_ty :=
-    fun i j => (e_from G j ==b i).
-
-  Definition inc_matrix_inv : inc_mat_ty :=
-    fun i j => (e_to G j ==b i).
-
-  Theorem inc_matrix_spec i j :
-    inc_matrix i j <->
-      e_from G j = i.
-  Proof.
-    unfold inc_matrix.
-    unfold is_true.
-    now rewrite equiv_decb_true_iff.
-  Qed.
-
-  Theorem inc_matrix_inv_spec i j :
-    inc_matrix_inv i j <->
-      e_to G j = i.
-  Proof.
-    unfold inc_matrix_inv.
-    unfold is_true.
-    now rewrite equiv_decb_true_iff.
-  Qed.
-
-  Theorem inc_matrix_spec_OUT i j :
-    inc_matrix i j <->
-      Path.matches_direction G i (e_to G j) j Pattern.OUT.
-  Proof.
-    rewrite inc_matrix_spec.
-    simpl; unfold e_from, e_to; destruct (ends G j); simpl.
-    split; ins; desf.
-  Qed.
-
-  Theorem inc_matrix_inv_spec_IN i j :
-    inc_matrix_inv i j <->
-      Path.matches_direction G i (e_from G j) j Pattern.IN.
-  Proof.
-    rewrite inc_matrix_inv_spec.
-    simpl; unfold e_from, e_to; destruct (ends G j); simpl.
-    split; ins; desf.
-  Qed.
-
   Definition label_matrix (l : label) : adj_mat_ty :=
     fun i j => eqb i j && In_decb l (vlabels G i).
 
-  Theorem label_matrix_spec l i j :
+  Lemma label_matrix_spec l i j :
     label_matrix l i j <-> i = j /\ In l (vlabels G i).
-  Proof.
+  Proof using.
     unfold label_matrix, is_true.
     rewrite Bool.andb_true_iff, In_decb_true_iff.
     case eqb_spec; split; ins; desf.
@@ -209,36 +165,61 @@ Section translate.
       in mpi' ⋅ mpe ⋅ mpv
     end.
 
+  Lemma end_In_V e u v
+    (HIn : In e E)
+    (Hends : ends G e = (u, v) \/ ends G e = (v, u)) :
+      In v V.
+  Proof using Hwf_G.
+    destruct Hwf_G. desf.
+    all: edestruct ends_In0; eauto.
+  Qed.
+
+  Lemma translate_slice'_hop_spec pi' pe pv i j :
+    translate_slice' (PatternSlice.hop pi' pe pv) i j <->
+      << HInV : In (j : vertex) V >> /\
+      exists k e,
+        << HInE : In e E >> /\
+        << Hik : translate_slice' pi' i k >> /\
+        << Hkj : Path.matches_direction G k j e (Pattern.edir pe) >> /\
+        << Helabel : match Pattern.elabel pe with
+                     | Some l => elabel G e = l
+                     | None => True
+                     end >> /\
+        << Hvlabel : match Pattern.vlabel pv with
+                     | Some l => In l (vlabels G j)
+                     | None => True
+                     end >>.
+  Proof using Hwf_G.
+    simpls.
+    repeat setoid_rewrite bmx_dot_spec.
+    destruct (Pattern.edir pe).
+    1: setoid_rewrite adj_matrix_spec_OUT.
+    2: setoid_rewrite adj_matrix_spec_IN.
+    3: setoid_rewrite adj_matrix_spec_BOTH.
+    all: destruct (Pattern.vlabel pv).
+    all: try setoid_rewrite label_matrix_spec.
+    all: try setoid_rewrite bmx_one_spec.
+    all: split; ins; desf; unnw; eauto 11 using end_In_V.
+  Qed.
+
   Theorem translate_slice'_spec' pi' i j r n_from
     (Hwf' : PatternSlice.wf' (Rcd.type_of r) pi')
     (Hij : translate_slice' pi' i j)
     (Hprev : r n_from = Some (Value.GVertex i)) :
-      exists p', PathSlice.matches G r n_from r p' pi' /\
-                  PathSlice.last r n_from p' = j.
+      exists p', << Hmatch : PathSlice.matches G r n_from r p' pi' >> /\
+                 << Hlast : PathSlice.last r n_from p' = j >>.
   Proof using Hwf_G.
     gen_dep j.
-    induction pi'; ins.
-    { exists PathSlice.empty. split.
+    induction pi'; intros.
+    { simpls. exists PathSlice.empty. split.
       { constructor. eexists; eassumption. }
       rewrite bmx_one_spec in Hij. simpl. desf. }
 
     inv Hwf'. inv Hwf_G.
 
-    repeat setoid_rewrite bmx_dot_spec in Hij.
-    destruct Hij as [j' [[k [Hik Hkj]] Hj'j]].
+    rewrite translate_slice'_hop_spec in Hij; desc.
     apply IHpi' in Hik; clear IHpi'; auto.
-
-    destruct (Pattern.vlabel pv) as [l |] eqn:Heq_v.
-    1: rewrite label_matrix_spec in Hj'j;
-        destruct Hj'j as [? Hvlabel].
-    2: rewrite bmx_one_spec in Hj'j.
-    all: subst j'.
-
-    all: destruct (Pattern.edir pe) eqn:Heq_edir; simpls.
-    all: try rewrite adj_matrix_spec_OUT in Hkj.
-    all: try rewrite adj_matrix_spec_IN in Hkj.
-    all: try rewrite adj_matrix_spec_BOTH in Hkj.
-    all: desf.
+    desf; unnw.
 
     all: exists (PathSlice.hop p' e j); split; [| reflexivity].
     all: replace r with ((Pattern.vname pv, Pattern.ename pe) |-[Mixed]->
@@ -249,10 +230,6 @@ Section translate.
                 eauto using PatternSlice.type_of_None).
     all: try constructor.
     all: try (ins; congruence).
-    all: try now rewrite Hik0, Heq_edir.
-
-    all: unfold Path.matches_direction in Hkj0; desf.
-    all: edestruct ends_In0; eauto.
   Qed.
 
   Theorem translate_slice'_spec r r' n_from p' pi' (i j : ord _) 
@@ -262,9 +239,9 @@ Section translate.
     (Hlast : PathSlice.last r n_from p' = j)
     (Hmatch : PathSlice.matches G r n_from r' p' pi') :
       translate_slice' pi' i j.
-  Proof.
-    gen_dep j; induction Hmatch; ins; subst.
-    { simpl. rewrite bmx_one_spec. desf. now apply eq_ord. }
+  Proof using Hwf_G.
+    gen_dep j; induction Hmatch; intros; subst.
+    { simpls. rewrite bmx_one_spec. desf. now apply eq_ord. }
 
     assert (exists k : ord vertices_sup, PathSlice.last r n_from p = k) as [k Hk].
     { enough (HIn : In (PathSlice.last r n_from p) (vertices G)).
@@ -275,35 +252,270 @@ Section translate.
     { apply IHHmatch; auto. inv Hwf'. }
     clear IHHmatch.
 
-    repeat setoid_rewrite bmx_dot_spec.
-    desf.
+    rewrite translate_slice'_hop_spec.
+    destruct Hpv, Hpe. simpls. subst.
+    split; auto.
 
-    all: exists j.
-    all: try rewrite bmx_one_spec.
-    all: try rewrite label_matrix_spec.
-    all: destruct Hpv.
-    all: splits; auto.
-
-    all: exists k.
-    all: split; [ assumption | ].
-
-    all: simpl.
-    all: match goal with
-          | [ _ : _ = Pattern.OUT |- _ ] =>
-              rewrite adj_matrix_spec_OUT
-          | [ _ : _ = Pattern.IN |- _ ] =>
-              rewrite adj_matrix_spec_IN
-          | [ _ : _ = Pattern.BOTH |- _ ] =>
-              rewrite adj_matrix_spec_BOTH
-          end.
-    all: exists e.
-    all: destruct Hpe.
-    all: rewrite Hk in Hdir.
-    all: splits; auto.
-    all: desf; eauto.
+    exists k. exists e.
+    splits; auto.
+    { now rewrite <- Hk. }
+    all: desf; auto.
   Qed.
-End translate.
 
+  Definition translate_slice (pi' : PatternSlice.t) : adj_mat_ty :=
+    translate_slice' pi'.
+
+  Theorem translate_slice_spec' pi' pe pv i j r n_from
+    (Hwf : PatternSlice.wf (Rcd.type_of r) (PatternSlice.hop pi' pe pv))
+    (Hij : translate_slice (PatternSlice.hop pi' pe pv) i j)
+    (Hprev_pv : r (Pattern.vname pv) = None \/
+                r (Pattern.vname pv) = Some (Value.GVertex j))
+    (Hprev : r n_from = Some (Value.GVertex i)) :
+      exists p' e, PathSlice.matches G r n_from
+                    ((Pattern.vname pv, Pattern.ename pe) |-[Mixed]->
+                     (Value.GVertex j, Value.GEdge e); r)
+                    (PathSlice.hop p' e j) (PatternSlice.hop pi' pe pv).
+  Proof using Hwf_G.
+    inv Hwf.
+    unfold translate_slice in Hij.
+    rewrite translate_slice'_hop_spec in Hij; desc.
+    eapply translate_slice'_spec' in Hik; eauto; desc.
+    rewrite <- Hlast in Hkj.
+
+    do 2 eexists.
+    econstructor; eauto.
+    all: constructor; ins; desf; auto.
+  Qed.
+
+  Theorem translate_slice_spec r r' n_from p' pi' (i j : ord _) 
+    (Hwf : PatternSlice.wf (Rcd.type_of r) pi')
+    (Hprev : r n_from = Some (Value.GVertex i))
+    (HIn_prev : In (i : vertex) (vertices G))
+    (Hlast : PathSlice.last r n_from p' = j)
+    (Hmatch : PathSlice.matches G r n_from r' p' pi') :
+      translate_slice pi' i j.
+  Proof using Hwf_G.
+    destruct Hmatch.
+    { simpls. rewrite bmx_one_spec. desf. now apply eq_ord. }
+
+    inv Hwf. destruct Hpv, Hpe.
+    unfold translate_slice.
+    rewrite translate_slice'_hop_spec; unnw.
+    simpls. subst.
+    split; [ assumption |].
+
+    assert (exists k : ord vertices_sup, PathSlice.last r n_from p = k) as [k Hk].
+    { enough (HIn : In (PathSlice.last r n_from p) (vertices G)).
+      now eexists (ord_of_vertex _ HIn).
+      eapply PathSlice.matches_last_In; eauto. }
+    rewrite Hk in Hdir.
+
+    exists k. exists e.
+    splits; auto.
+    { eapply translate_slice'_spec; eauto. }
+    all: desf; auto.
+  Qed.
+
+  Definition inc_mat_ty := bmx vertices_sup edges_sup.
+
+  Definition inc_matrix (l : option label) : inc_mat_ty :=
+    fun i j => (e_from G j ==b i) &&
+               match l with
+               | Some l => (elabel G j ==b l)
+               | None => true
+               end.
+
+  Definition inc_matrix_inv (l : option label) : inc_mat_ty :=
+    fun i j => (e_to G j ==b i) &&
+               match l with
+               | Some l => (elabel G j ==b l)
+               | None => true
+               end.
+
+  Theorem inc_matrix_spec l i j :
+    inc_matrix l i j <->
+      e_from G j = i /\
+      match l with
+      | Some l => (elabel G j = l)
+      | None => True
+      end.
+  Proof using.
+    unfold inc_matrix, is_true.
+    rewrite Bool.andb_true_iff.
+    desf.
+    all: now repeat rewrite equiv_decb_true_iff.
+  Qed.
+
+  Theorem inc_matrix_inv_spec l i j :
+    inc_matrix_inv l i j <->
+      e_to G j = i /\
+      match l with
+      | Some l => (elabel G j = l)
+      | None => True
+      end.
+  Proof using.
+    unfold inc_matrix_inv, is_true.
+    rewrite Bool.andb_true_iff.
+    desf.
+    all: now repeat rewrite equiv_decb_true_iff.
+  Qed.
+
+  Theorem inc_matrix_spec_OUT l i j :
+    inc_matrix l i j <->
+      Path.matches_direction G i (e_to G j) j Pattern.OUT /\
+      match l with
+      | Some l => (elabel G j = l)
+      | None => True
+      end.
+  Proof using.
+    rewrite inc_matrix_spec.
+    simpl; unfold e_from, e_to; destruct (ends G j); simpl.
+    split; ins; desf.
+  Qed.
+
+  Theorem inc_matrix_inv_spec_IN l i j :
+    inc_matrix_inv l i j <->
+      Path.matches_direction G i (e_from G j) j Pattern.IN /\
+      match l with
+      | Some l => (elabel G j = l)
+      | None => True
+      end.
+  Proof using.
+    rewrite inc_matrix_inv_spec.
+    simpl; unfold e_from, e_to; destruct (ends G j); simpl.
+    split; ins; desf.
+  Qed.
+
+  Definition e_from_dir (d : Pattern.direction) (e : edge) : vertex :=
+    match d with
+    | Pattern.OUT => e_to G e
+    | Pattern.IN => e_from G e
+    | Pattern.BOTH => 0%nat (* should not be used *)
+    end.
+  
+  Definition inc_label_matrix l d : bmx edges_sup edges_sup :=
+    fun e e' => eqb e e' && In_decb l (vlabels G (e_from_dir d e)).
+
+  Lemma inc_label_matrix_spec l (e e' : ord _) d :
+    let j := e_from_dir d e in
+      inc_label_matrix l d e e' <->
+        e = e' /\ In l (vlabels G (e_from_dir d e)).
+  Proof using.
+    unfold inc_label_matrix, is_true.
+    rewrite Bool.andb_true_iff, In_decb_true_iff.
+    case eqb_spec; split; ins; desf.
+  Qed.
+
+  Definition translate_slice_inc (pi' : PatternSlice.t) : inc_mat_ty :=
+    match pi' with
+    | PatternSlice.empty => 0
+    | PatternSlice.hop pi' pe pv =>
+      let mpi' := translate_slice' pi' in
+      let mpe :=
+        let l := Pattern.elabel pe in
+          match Pattern.edir pe with
+          | Pattern.OUT => inc_matrix l
+          | Pattern.IN => inc_matrix_inv l
+          | Pattern.BOTH => 0 (* should not be used *)
+          end
+      in
+      let mpv := 
+        match Pattern.vlabel pv with
+        | Some l => inc_label_matrix l (Pattern.edir pe)
+        | None => 1 (* identity matrix *)
+        end
+      in mpi' ⋅ mpe ⋅ mpv
+    end.
+
+  Lemma translate_slice_inc_hop_spec pi' pe pv i (e : ord _) :
+    let j := e_from_dir (Pattern.edir pe) e in
+      translate_slice_inc (PatternSlice.hop pi' pe pv) i e <->
+        exists k,
+          << Hik : translate_slice' pi' i k >> /\
+          << Hkj : match Pattern.edir pe with
+                   | Pattern.OUT => Path.matches_direction G k j e Pattern.OUT
+                   | Pattern.IN => Path.matches_direction G k j e Pattern.IN
+                   | Pattern.BOTH => False
+                   end >> /\
+          << Helabel : match Pattern.elabel pe with
+                       | Some l => elabel G e = l
+                       | None => True
+                       end >> /\
+          << Hvlabel : match Pattern.vlabel pv with
+                       | Some l => In l (vlabels G j)
+                       | None => True
+                       end >>.
+  Proof using.
+    simpl.
+    repeat setoid_rewrite bmx_dot_spec.
+    destruct (Pattern.edir pe), (Pattern.vlabel pv).
+    all: try setoid_rewrite inc_matrix_spec_OUT.
+    all: try setoid_rewrite inc_matrix_inv_spec_IN.
+    all: try setoid_rewrite bmx_one_spec.
+    all: try setoid_rewrite label_matrix_spec.
+    all: try setoid_rewrite inc_label_matrix_spec.
+    all: simpls.
+    all: split; ins; desf; eauto 12.
+  Qed.
+
+  Section translate_slice_inc_spec.
+    Variable pi' : PatternSlice.t.
+    Variable pe : Pattern.pedge.
+    Variable pv : Pattern.pvertex.
+    Variable i : ord vertices_sup.
+    Variable e : ord edges_sup.
+    Variable r : Rcd.t.
+    Variable n_from : Name.t.
+
+    Notation j := (e_from_dir (Pattern.edir pe) e).
+
+    Hypothesis Hwf : PatternSlice.wf (Rcd.type_of r) (PatternSlice.hop pi' pe pv).
+    Hypothesis HIn_e : In (e : edge) (edges G).
+    
+    Theorem translate_slice_inc_spec'
+      (Hij : translate_slice_inc (PatternSlice.hop pi' pe pv) i e)
+      (Hprev_pv : r (Pattern.vname pv) = None \/
+                  r (Pattern.vname pv) =
+                    Some (Value.GVertex j))
+      (Hprev : r n_from = Some (Value.GVertex i)) :
+        exists p', PathSlice.matches G r n_from
+                    ((Pattern.vname pv, Pattern.ename pe) |-[Mixed]->
+                      (Value.GVertex j, Value.GEdge e); r)
+                    (PathSlice.hop p' e j) (PatternSlice.hop pi' pe pv).
+    Proof using Hwf_G Hwf HIn_e.
+      inv Hwf.
+      apply translate_slice_inc_hop_spec in Hij; desc.
+      eapply translate_slice'_spec' in Hik; eauto; desc.
+      rewrite <- Hlast in Hkj.
+      exists p'; constructor; auto.
+      all: destruct (Pattern.edir pe); simpls.
+      all: constructor; auto using wf_e_from_In, wf_e_to_In.
+      all: ins; desf; auto 2.
+    Qed.
+
+    Theorem translate_slice_inc_spec p' r'
+      (Hprev : r n_from = Some (Value.GVertex i))
+      (HIn_prev : In (i : vertex) (vertices G))
+      (Hdir : Pattern.edir pe = Pattern.OUT \/ Pattern.edir pe = Pattern.IN)
+      (Hmatch : PathSlice.matches G r n_from r'
+                  (PathSlice.hop p' e j) (PatternSlice.hop pi' pe pv)) :
+        translate_slice_inc (PatternSlice.hop pi' pe pv) i e.
+    Proof using Hwf_G Hwf.
+      apply translate_slice_inc_hop_spec; unnw.
+      inv Hwf. inv Hmatch.
+
+      assert (exists k : ord vertices_sup, PathSlice.last r n_from p' = k) as [k Hk].
+      { enough (HIn : In (PathSlice.last r n_from p') (vertices G)).
+        now eexists (ord_of_vertex _ HIn).
+        eapply PathSlice.matches_last_In; eauto. }
+      do 2 eexists; splits.
+      { erewrite translate_slice'_spec; eauto. }
+      all: destruct Hpv, Hpe.
+      all: try rewrite <- Hk.
+      all: desf; auto.
+    Qed.
+  End translate_slice_inc_spec.
+End translate.
 
 Definition traverse : PatternSlice.t -> Name.t -> step1.
 Admitted.
